hide CBOR.Pulse.API.Det.C under an interface

src/cbor/pulse/CBOR.Pulse.API.Det.C.fst
@@ -1,38 +1,13 @@
 module CBOR.Pulse.API.Det.C
-include CBOR.Pulse.API.Det.Common
-open Pulse.Lib.Pervasives
-open CBOR.Spec.Constants
-
-module Spec = CBOR.Spec.API.Format
-module S = Pulse.Lib.Slice
-module A = Pulse.Lib.Array
-module PM = Pulse.Lib.SeqMatch
-module Trade = Pulse.Lib.Trade.Util
-module SZ = FStar.SizeT
-module U64 = FStar.UInt64
-module U8 = FStar.UInt8
 
 ```pulse
-fn cbor_det_mk_string_from_array
+fn cbor_det_mk_string_from_array (_: unit) : cbor_det_mk_string_from_array_t
+=
   (ty: major_type_byte_string_or_text_string)
   (a: A.array U8.t)
   (len: U64.t)
   (#p: perm)
   (#v: Ghost.erased (Seq.seq U8.t))
-requires
-    (pts_to a #p v ** pure (
-      Seq.length v == U64.v len /\
-      (ty == cbor_major_type_text_string ==> CBOR.Spec.API.UTF8.correct v)
-    ))
-returns res: cbor_det_t
-ensures
-    (exists* p' v' .
-      cbor_det_match p' res (Spec.pack (Spec.CString ty v')) **
-      Trade.trade
-        (cbor_det_match p' res (Spec.pack (Spec.CString ty v')))
-        (pts_to a #p v) **
-      pure (Ghost.reveal v == v')
-    )
 {
   A.pts_to_len a;
   let _ : squash (SZ.fits_u64) = assume SZ.fits_u64;
@@ -53,29 +28,14 @@ ensures
 ```
 
 ```pulse
-fn cbor_det_mk_array_from_array
+fn cbor_det_mk_array_from_array (_: unit) : cbor_det_mk_array_from_array_t
+=
   (a: A.array cbor_det_t)
   (len: U64.t)
   (#pa: perm)
   (#va: Ghost.erased (Seq.seq cbor_det_t))
   (#pv: perm)
   (#vv: Ghost.erased (list Spec.cbor))
-requires
-    (A.pts_to a #pa va **
-      PM.seq_list_match va vv (cbor_det_match pv) **
-      pure (A.length a == U64.v len)
-    )
-returns res: cbor_det_t
-ensures
-    (exists* p' v' .
-      cbor_det_match p' res (Spec.pack (Spec.CArray v')) **
-      Trade.trade
-        (cbor_det_match p' res (Spec.pack (Spec.CArray v')))
-        (A.pts_to a #pa va **
-          PM.seq_list_match va vv (cbor_det_match pv)
-        ) **
-        pure (Ghost.reveal vv == v')
-    )
 {
   A.pts_to_len a;
   let _ : squash (SZ.fits_u64) = assume SZ.fits_u64;
@@ -97,33 +57,13 @@ ensures
 ```
 
 ```pulse
-fn cbor_det_mk_map_from_array
+fn cbor_det_mk_map_from_array (_: unit) : cbor_det_mk_map_from_array_t
+=
   (a: A.array cbor_det_map_entry_t)
   (len: U64.t)
   (#va: Ghost.erased (Seq.seq cbor_det_map_entry_t))
   (#pv: perm)
   (#vv: Ghost.erased (list (Spec.cbor & Spec.cbor)))
-requires
-    (A.pts_to a va **
-      PM.seq_list_match va vv (cbor_det_map_entry_match pv) **
-      pure (A.length a == U64.v len /\
-        List.Tot.no_repeats_p (List.Tot.map fst vv)
-      )
-    )
-returns res: cbor_det_t
-ensures
-    (exists* p' v' va' .
-      cbor_det_match p' res (Spec.pack (Spec.CMap v')) **
-      Trade.trade
-        (cbor_det_match p' res (Spec.pack (Spec.CMap v')))
-        (A.pts_to a va' **
-          PM.seq_list_match va vv (cbor_det_map_entry_match pv)
-        ) **
-        pure (
-          (forall x . List.Tot.assoc x vv == Spec.cbor_map_get v' x) /\
-          Spec.cbor_map_length v' == Seq.length va
-        )
-    )
 {
   A.pts_to_len a;
   let _ : squash (SZ.fits_u64) = assume SZ.fits_u64;
