src/cbor/pulse/CBOR.Pulse.API.Det.C.fsti
@@ -1,0 +1,99 @@
+module CBOR.Pulse.API.Det.C
+include CBOR.Pulse.API.Det.Common
+open Pulse.Lib.Pervasives
+open CBOR.Spec.Constants
+
+module Spec = CBOR.Spec.API.Format
+module S = Pulse.Lib.Slice
+module A = Pulse.Lib.Array
+module PM = Pulse.Lib.SeqMatch
+module Trade = Pulse.Lib.Trade.Util
+module SZ = FStar.SizeT
+module U64 = FStar.UInt64
+module U8 = FStar.UInt8
+
+inline_for_extraction
+noextract [@@noextract_to "krml"]
+let cbor_det_mk_string_from_array_t =
+  (ty: major_type_byte_string_or_text_string) ->
+  (a: A.array U8.t) ->
+  (len: U64.t) ->
+  (#p: perm) ->
+  (#v: Ghost.erased (Seq.seq U8.t)) ->
+  stt cbor_det_t
+    (pts_to a #p v ** pure (
+      Seq.length v == U64.v len /\
+      (ty == cbor_major_type_text_string ==> CBOR.Spec.API.UTF8.correct v)
+    ))
+    (fun res -> exists* p' v' .
+      cbor_det_match p' res v' **
+      Trade.trade
+        (cbor_det_match p' res v')
+        (pts_to a #p v) **
+      pure (
+        Spec.CString? (Spec.unpack v') /\
+        Ghost.reveal v == Spec.CString?.v (Spec.unpack v')
+      )
+    )
+
+val cbor_det_mk_string_from_array (_: unit) : cbor_det_mk_string_from_array_t
+
+inline_for_extraction
+noextract [@@noextract_to "krml"]
+let cbor_det_mk_array_from_array_t =
+  (a: A.array cbor_det_t) ->
+  (len: U64.t) ->
+  (#pa: perm) ->
+  (#va: Ghost.erased (Seq.seq cbor_det_t)) ->
+  (#pv: perm) ->
+  (#vv: Ghost.erased (list Spec.cbor)) ->
+  stt cbor_det_t
+    (A.pts_to a #pa va **
+      PM.seq_list_match va vv (cbor_det_match pv) **
+      pure (A.length a == U64.v len)
+    )
+    (fun res -> exists* p' v' .
+      cbor_det_match p' res v' **
+      Trade.trade
+        (cbor_det_match p' res v')
+        (A.pts_to a #pa va **
+          PM.seq_list_match va vv (cbor_det_match pv)
+        ) **
+        pure (
+          Spec.CArray? (Spec.unpack v') /\
+          Ghost.reveal vv == Spec.CArray?.v (Spec.unpack v')
+        )
+    )
+
+val cbor_det_mk_array_from_array (_: unit) : cbor_det_mk_array_from_array_t
+
+inline_for_extraction
+noextract [@@noextract_to "krml"]
+let cbor_det_mk_map_from_array_t =
+  (a: A.array cbor_det_map_entry_t) ->
+  (len: U64.t) ->
+  (#va: Ghost.erased (Seq.seq cbor_det_map_entry_t)) ->
+  (#pv: perm) ->
+  (#vv: Ghost.erased (list (Spec.cbor & Spec.cbor))) ->
+  stt cbor_det_t
+    (A.pts_to a va **
+      PM.seq_list_match va vv (cbor_det_map_entry_match pv) **
+      pure (A.length a == U64.v len /\
+        List.Tot.no_repeats_p (List.Tot.map fst vv)
+      )
+    )
+    (fun res -> exists* p' v' va' .
+      cbor_det_match p' res v' **
+      Trade.trade
+        (cbor_det_match p' res v')
+        (A.pts_to a va' **
+          PM.seq_list_match va vv (cbor_det_map_entry_match pv)
+        ) **
+        pure (
+          Spec.CMap? (Spec.unpack v') /\
+          (forall x . List.Tot.assoc x vv == Spec.cbor_map_get (Spec.CMap?.c (Spec.unpack v')) x) /\
+          Spec.cbor_map_length (Spec.CMap?.c (Spec.unpack v')) == Seq.length va
+        )
+    )
+
+val cbor_det_mk_map_from_array (_: unit) : cbor_det_mk_map_from_array_t
